Port proofs

CC/Subcapt/Basic.lean
@@ -13,6 +13,13 @@ namespace CC
 def Subcapt.refl :
   Subcapt Γ C C := by
   apply Subcapt.sc_set
-  intro x0 h
-  apply Subcapt.sc_elem
-  aesop
+  · intro x0 h
+    apply Subcapt.sc_elem
+    aesop
+  · intro x0 h
+    apply Subcapt.sc_elem_reach
+    aesop
+  · intro h
+    unfold CaptureSet.isUniversal at h
+    cases C; cases h
+    apply Subcapt.sc_elem_cap
