CC/Typed.lean
@@ -21,31 +21,28 @@ def Variance.neg : Variance -> Variance
 | Variance.cov => Variance.cot
 | Variance.cot => Variance.cov
 
-def CaptureSet.refine_reach (C : CaptureSet n) (x : Fin n) (v : Variance) : CaptureSet n :=
-  match C.hasCap, v with
-  | false, _ => C
-  | true, Variance.cov => ⟨C.elems, C.reachElems ∪ {x}, false⟩
-  | true, Variance.cot => C
+inductive RefineCaptureSet : CaptureSet n -> Fin n -> Variance -> CaptureSet n -> Prop where
+| pos :
+  RefineCaptureSet ⟨cs, rs, u⟩ x Variance.cov ⟨∅, rs ∪ {x}, false⟩
+| neg :
+  RefineCaptureSet ⟨cs, rs, u⟩ x Variance.cot ⟨cs, rs, u⟩
 
-def PType.refine_reach (S : PType n m) (x : Fin n) (v : Variance) : PType n m :=
-  match S with
-  | PType.tvar _ => S
-  | PType.top => S
-  | PType.arr (CType.capt C S) U => PType.arr (CType.capt (C.refine_reach x v.neg) (S.refine_reach x v)) U
-  | PType.tarr R (CType.capt C S) => PType.tarr R (CType.capt (C.refine_reach x v) (S.refine_reach x v))
-  | PType.boxed (CType.capt C S) => PType.boxed (CType.capt (C.refine_reach x v) (S.refine_reach x v))
-
-@[simp]
-theorem refine_reach_boxed :
-  (PType.boxed (CType.capt C S)).refine_reach x v = PType.boxed (CType.capt (C.refine_reach x v) (S.refine_reach x v)) := by simp [PType.refine_reach]
-
-@[simp]
-theorem refine_reach_arr :
-  (PType.arr (CType.capt C S) U).refine_reach x v = PType.arr (CType.capt (C.refine_reach x v.neg) (S.refine_reach x v)) U := by simp [PType.refine_reach]
-
-@[simp]
-theorem refine_reach_tarr :
-  (PType.tarr R (CType.capt C S)).refine_reach x v = PType.tarr R (CType.capt (C.refine_reach x v) (S.refine_reach x v)) := by simp [PType.refine_reach]
+inductive RefinePType : PType n m -> Fin n -> Variance -> PType n m -> Prop where
+| identity : RefinePType S x v S
+| tvar : RefinePType (PType.tvar X) x v (PType.tvar X)
+| top : RefinePType PType.top x v PType.top
+| arr :
+  RefineCaptureSet C x v.neg C' ->
+  RefinePType S x v.neg S' ->
+  RefinePType (PType.arr (CType.capt C S) U) x v (PType.arr (CType.capt C' S) U)
+| tarr :
+  RefineCaptureSet C x v C' ->
+  RefinePType S x v S' ->
+  RefinePType (PType.tarr R (CType.capt C S)) x v (PType.tarr R (CType.capt C' S))
+| boxed :
+  RefineCaptureSet C x v C' ->
+  RefinePType S x v S' ->
+  RefinePType (PType.boxed (CType.capt C S)) x v (PType.boxed (CType.capt C' S))
 
 inductive DropBinderFree : CaptureSet n.succ -> CaptureSet n -> Prop where
   | drop : DropBinderFree C.weaken_var C
@@ -57,7 +54,11 @@ inductive DropBinder : CaptureSet n.succ -> CaptureSet n -> Prop where
 inductive Typed : Ctx n m -> Term n m -> CaptureSet n -> CType n m -> Prop where
 | var :
   BoundVar Γ x (CType.capt C S) ->
-  Typed Γ (Term.var x) {x} (CType.capt {x} (S.refine_reach x Variance.cov))
+  Typed Γ (Term.var x) {x} (CType.capt {x} S)
+| var_refine :
+  Typed Γ (Term.var x) {x} (CType.capt C S) ->
+  RefinePType S x Variance.cov S' ->
+  Typed Γ (Term.var x) {x} (CType.capt C S')
 | sub :
   Typed Γ t C T ->
   Subtype Γ T T' ->
