CC/Typed/Rename.lean
@@ -32,49 +32,47 @@ def DropBinder.rename (h : DropBinder C C') :
     rw [<- CaptureSet.rename_weaken_comm]
     apply DropBinder.drop
 
--- def RefineCaptureSet.rename (h : RefineCaptureSet C x v C') :
---   RefineCaptureSet (C.rename f) (f x) v (C'.rename f) := by
---   induction h
---   case pos_nocap => simp [CaptureSet.rename]; constructor
---   case pos_cap => simp [CaptureSet.rename, Finset.image_union]; constructor
---   case neg => constructor
+def RefineCaptureSet.rename (h : RefineCaptureSet C x v C') :
+  RefineCaptureSet (C.rename f) (f x) v (C'.rename f) := by
+  induction h
+  case pos => simp [CaptureSet.rename, Finset.image_union]; constructor
+  case neg => constructor
 
-theorem CaptureSet.rename_refine_reach {C : CaptureSet n} :
-  (C.refine_reach x v).rename f = (C.rename f).refine_reach (f x) v := by
-  cases C; rename_i u; cases u <;> try (solve | simp [rename, refine_reach])
-  cases v <;> simp [rename, refine_reach, Finset.image_union]
+-- theorem CaptureSet.rename_refine_reach {C : CaptureSet n} :
+--   (C.refine_reach x v).rename f = (C.rename f).refine_reach (f x) v := by
+--   cases C; rename_i u; cases u <;> try (solve | simp [rename, refine_reach])
+--   cases v <;> simp [rename, refine_reach, Finset.image_union]
 
--- def RefinePType.rename (h : RefinePType S x v S') :
---   RefinePType (S.rename f g) (f x) v (S'.rename f g) := by
---   rename_i n1 m1 n2 m2
---   induction h generalizing n2 m2 <;> try (solve | simp [PType.rename]; constructor)
---   case arr =>
---     simp [PType.rename]; constructor
---     aesop
---     apply RefineCaptureSet.rename; trivial
---   case tarr =>
---     simp [PType.rename]; constructor
---     aesop; apply RefineCaptureSet.rename; trivial
---   case boxed =>
---     simp [PType.rename]; constructor
---     aesop; apply RefineCaptureSet.rename; trivial
+def RefinePType.rename (h : RefinePType S x v S') :
+  RefinePType (S.rename f g) (f x) v (S'.rename f g) := by
+  rename_i n1 m1 n2 m2
+  induction h generalizing n2 m2 <;> try (solve | simp [PType.rename]; constructor)
+  case arr =>
+    simp [PType.rename]; constructor
+    apply RefineCaptureSet.rename; trivial; aesop
+  case tarr =>
+    simp [PType.rename]; constructor
+    apply RefineCaptureSet.rename; trivial; aesop
+  case boxed =>
+    simp [PType.rename]; constructor
+    apply RefineCaptureSet.rename; trivial; aesop
 
-def PType.rename_refine_reach : (S : PType n m) ->
-  (S.refine_reach x v).rename f g = (S.rename f g).refine_reach (f x) v
-| PType.tvar X => by simp [rename, refine_reach]
-| PType.top => by simp [rename, refine_reach]
-| PType.boxed (CType.capt C S) => by
-  simp
-  simp [CaptureSet.rename_refine_reach]
-  apply PType.rename_refine_reach
-| PType.arr (CType.capt C S) U => by
-  simp
-  simp [CaptureSet.rename_refine_reach]
-  apply PType.rename_refine_reach
-| PType.tarr R (CType.capt C S) => by
-  simp
-  simp [CaptureSet.rename_refine_reach]
-  apply PType.rename_refine_reach
+-- def PType.rename_refine_reach : (S : PType n m) ->
+--   (S.refine_reach x v).rename f g = (S.rename f g).refine_reach (f x) v
+-- | PType.tvar X => by simp [rename, refine_reach]
+-- | PType.top => by simp [rename, refine_reach]
+-- | PType.boxed (CType.capt C S) => by
+--   simp
+--   simp [CaptureSet.rename_refine_reach]
+--   apply PType.rename_refine_reach
+-- | PType.arr (CType.capt C S) U => by
+--   simp
+--   simp [CaptureSet.rename_refine_reach]
+--   apply PType.rename_refine_reach
+-- | PType.tarr R (CType.capt C S) => by
+--   simp
+--   simp [CaptureSet.rename_refine_reach]
+--   apply PType.rename_refine_reach
 
 def Typed.rename {Γ : Ctx n1 m1} (h : Typed Γ t C T)
   {Δ : Ctx n2 m2}
@@ -85,11 +83,16 @@ def Typed.rename {Γ : Ctx n1 m1} (h : Typed Γ t C T)
   case var =>
     simp [Term.rename]
     rename_i hb
-    simp [PType.rename_refine_reach]
     apply Typed.var
     have hb' := σ hb
     simp [CType.rename] at hb'
     exact hb'
+  case var_refine =>
+    simp [Term.rename]
+    apply Typed.var_refine
+    rename_i ih
+    apply ih <;> trivial
+    apply RefinePType.rename; trivial
   case sub =>
     apply Typed.sub
     aesop
