CC/Subcapt/Subst.lean
@@ -29,13 +29,26 @@ def Subcapt.subst (σ : VarSubst Γ Δ f) :
     have h' := σ h
     simp [CType.rename] at h'
     apply Typed.var_inv_subcapt; aesop
-  case sc_set hs =>
+  case sc_set hs hr hu =>
     apply Subcapt.sc_set
-    intro x1 h1
-    rw [mem_rename] at h1
-    let ⟨x2, ⟨h2, eq2⟩⟩ := h1
-    have h := hs x2 h2 σ
-    rw [rename_singleton] at h
-    rw [<- eq2]
-    assumption
+    · intro x1 h1
+      rw [mem_rename] at h1
+      let ⟨x2, ⟨h2, eq2⟩⟩ := h1
+      have h := hs x2 h2 σ
+      rw [rename_singleton] at h
+      rw [<- eq2]
+      assumption
+    · intro x1 h1
+      rw [mem_reach_rename] at h1
+      let ⟨x2, ⟨h2, eq2⟩⟩ := h1
+      have h := hr x2 h2 σ
+      rw [rename_singleton_reach] at h
+      rw [<- eq2]
+      assumption
+    · intro hc; aesop
   case sc_reach => simp; apply Subcapt.sc_reach
+  case sc_elem_cap => simp; simp [CaptureSet.rename]; apply Subcapt.sc_elem_cap
+  case sc_elem_reach =>
+    simp; apply Subcapt.sc_elem_reach
+    apply mem_rename_of_mem_reach; assumption
+  case sc_reach_cap => simp; apply Subcapt.sc_reach_cap
